Superposition_Calculus/Term_Rewrite_System.thy
@@ -1,6 +1,5 @@
 theory Term_Rewrite_System
   imports
-    Isabelle_2024_Compatibility
     Regular_Tree_Relations.Ground_Ctxt
 begin
 
